\begin{align*}
	&\left\{\begin{array}{@{}>{\displaystyle}l@{}}
		A e^{ikR} + B e^{-ikR} = C e^{-qR} \\
		ik A e^{ikR} - ik B e^{-ikR} = - q C e^{-qR}
	\end{array}\right. 
	\iff
	\left\{\begin{array}{@{}>{\displaystyle}l@{}}
		A (e^{ikR} - e^{-ikR} ) = C e^{-qR} \\
		ik A (e^{ikR} + e^{-ikR}) = - q C e^{-qR}
	\end{array}\right.\\
	&\iff
	ik A (e^{ikR} + e^{-ikR}) + qA (e^{ikR} - e^{-ikR}) = 0
\end{align*}


and $u_\mathrm{I}'(R) = u_\mathrm{II}'(R)$.

\begin{align*}
	&\left\{\begin{array}{@{}>{\displaystyle}l@{}}
		A \sin{kR} = C e^{-qR} \\
		k A \cos{kR} = - q C e^{-qR}
	\end{array}\right.
	\iff
	A(k \cos{kR} + q\sin{kR}) = 0
\end{align*}